### Description:
This code does not execute properly. Try to figure out why.

\#Debugging \#Fundamentals

### Solutions

#### C 

```C
int multiply(int a, int b) {
  return (a*b);
}
```

```C
__asm__
(
    ".global multiply\n"
    "multiply:\n"
    "movl %edi, %eax\n"
    "mull %esi\n"
    "ret\n"
);
```

```C
const long multiply = 0xC3EEF7F889;
```

```C
int multiply(int a, char *b) {
  //get the address of b and dereference to get the value
  //assign it to an signed int to work with negative numbers
  int _b = &*b;
  return a * _b;
}
```

```C
const double multiply = 18117629973988060449308518964918467752448300643542725371361122020537593562421864700213872973439671302938629031182012696940773376.0;

/*
The user code and the tests code are in different files. All the linker cares about is that there is something called multiply associated with a callable piece of code. 18117629973988060449308518964918467752448300643542725371361122020537593562421864700213872973439671302938629031182012696940773376.0

is an IEEE754 double number represented in memory by the following bytes (little-endian, hexadecimal notation):

89 F8 0F AF C6 C3 5A 5A
Dissasembling these bytes, we get the following x64 assembly code:

0x89 0xF8      -> mov   eax,edi
0x0F 0xAF 0xC6 -> imul  eax,esi
0xC3           -> ret
0x5A           -> pop  rdx
0x5A           -> pop  rdx
which multiplies the integers in the edi an esi registers and puts the result in the register eax (following the System V AMD64 ABI that Linux uses)
*/
```

```C
#define Hey int multiply
#define I ( int a
#define just ,
#define met int b
#define you ) {
#define and return
#define this a *
#define is b;
#define crazy }

Hey I just met you and this is crazy
```


```C
int multiply(int a, int b){
  __asm__ ("imull %%eax, %%ebx;": "=b"(a): "a"(a), "b"(b));
  return a;
}
```

#### λ Calculus

```λ Calculus
multiply = \ m n x . m (n x)
```

$$
\begin{aligned}
\text{multiply} = \lambda m . \lambda n . \lambda x . m (n \, x)
\end{aligned}
$$

```λ Calculus
succ = \ n f x . f (n f x)
plus = \ m n . m succ n
multiply = \ m n . m (plus n) 0
```
$$
\begin{aligned}
\text{succ} &= \lambda n . \lambda f . \lambda x . f (n \, f \, x) \\
\text{plus} &= \lambda m . \lambda n . m \, \text{succ} \, n \\
\text{multiply} &= \lambda m . \lambda n . m (\text{plus} \, n) \, 0
\end{aligned}
$$
